coq-osiris/theories/program_logic/tactics.v
@@ -1,7 +1,6 @@
 From iris.proofmode Require Import tactics.
-
-From osiris.program_logic Require Import ewp.
 From osiris.semantics Require Import step code.
+From osiris.program_logic Require Import wp_step ewp.
 
 From Ltac2 Require Import Ltac2.
 
@@ -19,11 +18,9 @@ Module ewp_rules_tactics.
   (* ------------------------------------------------------------------------ *)
   (* Working with the state interpretation invariant. *)
 
-  (* [intro_state] introduces [σ] and [state_interp σ]. *)
+  (* [intro_state] introduces [σ], [π] and [state_interp (σ, π)]. *)
 
-  Ltac intro_state := iIntros (σ) "Hsi".
-
-  Ltac intro_thread := iIntros (π); try iIntros (?); iIntros "Hti".
+  Ltac intro_state := iIntros (σ π) "Hsi".
 
   (* -------------------------------------------------------------------------- *)
   (** * Modality and mask (fupd) tactics *)
@@ -80,10 +77,10 @@ Module ewp_rules_tactics.
     ewp_cleanup_mod.
 
   (* ------------------------------------------------------------------------ *)
-  (* [intro_step] introduces [prim_step] along with the new expression and state *)
+  (* [intro_step] introduces [wp_step] along with the new expression and state *)
   Ltac intro_step :=
     let Hstep := fresh "Hstep" in
-    iIntros (???Hstep).
+    iIntros (???? Hstep).
 
   (* Discharge pure subgoal that follows immediately by [tac] *)
   Tactic Notation "discharge_pure" tactic(tac) :=
@@ -94,9 +91,13 @@ Module ewp_rules_tactics.
         iSplitL ""; [ | iPureIntro; by tac ]
     end.
 
+  Ltac prove_can_wp_step :=
+    (auto with step can_wp_step) ||
+    (apply can_step_wp_step; auto with step can_step).
+
   Ltac construct_wp_nonret :=
     (* Prove [can_step]: *)
-    (discharge_pure (auto with step can_step));
+    (discharge_pure prove_can_wp_step);
     (* Introduce a hypothetical step: *)
     intro_step.
 
@@ -129,7 +130,7 @@ Module ewp_rules_tactics.
         intros ?; intros_until_ewp_case hm
     end.
 
-  Ltac2 destruct_prim_step () := ltac1:(destruct_prim_step).
+  Ltac2 destruct_wp_step () := ltac1:(destruct_wp_step).
 
   Ltac2 ewp_case (m : constr)  :=
     ltac1:(m |- case_eq (is_ewp_case m)) (Ltac1.of_constr m);
@@ -143,7 +144,7 @@ Module ewp_rules_tactics.
               destruct $m; try0 destruct_stop_code; try discriminate;
               Control.enter
                 (fun _ =>
-                   try (complete destruct_prim_step))))
+                   try (complete destruct_wp_step))))
       [ fun _ => let hm := Fresh.in_goal @Hhm in intros $hm ].
 
   Tactic Notation "ewp_case" constr(x)  :=
@@ -155,7 +156,7 @@ Module ewp_rules_tactics.
     | |- context
           [environments.Esnoc _ ?Hwp
              (bi_forall (fun σ1 : step.store =>
-              bi_forall (fun π1 : step.threadpool => _)))] =>
+              bi_forall (fun π1 : threadpool => _)))] =>
         match goal with
         | |- context [environments.Esnoc _ ?SI (bi_sep (osiris_state_interp ?σ) (osiris_thread_interp ?π))] =>
             let Hstep := fresh "Hstep" in
@@ -168,16 +169,16 @@ Module ewp_rules_tactics.
   (* Specialize hypothesis that expects a [step] relation and extract out
     information *)
   Ltac spec_step :=
-    match goal with
+    lazymatch goal with
     | |- context
           [environments.Esnoc _ ?Hwp
              (bi_forall (fun σ'0 =>
               bi_forall (fun π'0 =>
               bi_forall (fun m' =>
               bi_forall (fun μ0 =>
-              bi_wand (bi_pure ((prim_step (pair (pair (pair ?σ ?π) ?m) ?ι) _))) _)))))] =>
-        match goal with
-        | [Hstep : prim_step (σ, π, m, ι) _ |- _] =>
+              bi_wand (bi_pure ((wp_step (pair (pair (pair ?σ ?π) ?m) ?ι) _))) _)))))] =>
+        lazymatch goal with
+        | [ Hstep : wp_step (σ, π, m, ι) _ |- _] =>
             (* Specialize step relation *)
             iSpecialize (Hwp $! _ _ _ _ Hstep);
             (* Destruct the hypothesis *)
